proof/SimSymbId.v
@@ -19,25 +19,7 @@ Require Import System.
 Set Implicit Arguments.
 
 
-Inductive sim_skenv (skenv0 skenv1: SkEnv.t): Prop :=
-| sim_skenv_intro
-    (NEXT: skenv0.(Genv.genv_next) = skenv1.(Genv.genv_next))
-    (SYMB: all1 (skenv0.(Genv.find_symbol) =1= skenv1.(Genv.find_symbol)))
-    (DEFS: all1 (skenv0.(Genv.find_def) =1= skenv1.(Genv.find_def)))
-    (PUBS: skenv0.(Genv.genv_public) = skenv1.(Genv.genv_public))
-.
-
-Goal sim_skenv = Genv.match_genvs eq.
-Proof.
-  apply Axioms.functional_extensionality; i.
-  apply Axioms.functional_extensionality; i.
-  apply AxiomsC.prop_ext.
-  split; i; inv H; econs; eauto.
-  - ii. unfold Genv.find_def in *. erewrite DEFS.
-    destruct ((Genv.genv_defs x0) ! b) eqn:T; econs; eauto.
-  - unfold Genv.find_def in *. i. specialize (mge_defs x1). inv mge_defs; ss.
-  - admit "".
-Qed.
+Definition sim_skenv (skenv0 skenv1: SkEnv.t): Prop := skenv0 = skenv1.
 
 Lemma sim_skenv_equiv
       skenv_src skenv_tgt
@@ -60,30 +42,9 @@ Lemma system_sim_skenv
 Proof.
   inv SIMSKENV.
   econs; eauto.
-  unfold System.skenv in *.
-  i. spc DEFS.
-  match goal with
-  | [ |- ?LHS = ?RHS ] => destruct RHS eqn:T
-  end.
-  { apply_all_once Genv_map_defs_def. des.
-    rewrite <- DEFS in *.
-    eapply_all_once Genv_map_defs_def_inv. erewrite FIND.
-    des_ifs.
-  }
-  match goal with
-  | [ |- ?LHS = ?RHS ] => destruct LHS eqn:T0
-  end; ss.
-  { apply_all_once Genv_map_defs_def. des.
-    rewrite DEFS in *.
-    eapply_all_once Genv_map_defs_def_inv. erewrite FIND in *.
-    des_ifs.
-  }
 Qed.
 
-Inductive sim_sk (u: unit) (sk_src sk_tgt: Sk.t): Prop :=
-| closed_intro
-    (SIM: match_program (fun _ => eq) eq sk_src sk_tgt)
-.
+Definition sim_sk (u: unit) (sk_src sk_tgt: Sk.t): Prop := sk_src = sk_tgt.
 
 Definition le: unit -> Sk.t -> Sk.t -> unit -> Prop := top4.
 
@@ -105,7 +66,9 @@ Proof.
   i.
   inv SIMSK. inv SIMSK0.
   SearchAbout TransfLink.
-  admit "this should hold".
+  esplits; ss; eauto.
+Unshelve.
+  all: ss.
 Qed.
 
 Lemma sim_sk_load_sim_skenv: forall
@@ -125,15 +88,7 @@ Proof.
   Print Genv.init_mem_transf.
   Print Genv.init_mem_transf_partial.
   About Genv.init_mem_match.
-  exploit (Genv.init_mem_match SIM); eauto. i. clarify.
-  esplits; eauto.
-  - econs; eauto.
-    + erewrite ! Genv.init_mem_genv_next; eauto.
-    + i. symmetry. apply (Genv.find_symbol_match SIM).
-    + ii. hexploit (Genv.find_def_match_2 SIM x0); eauto. intro REL.
-      inv REL; ss. inv H2; ss.
-      * inv H3; ss.
-    + inv SIM; des; ss. rewrite ! Genv.globalenv_public. ss.
+  esplits; eauto. rr. ss.
 Qed.
 
 Lemma sim_skenv_monotone: forall
@@ -145,61 +100,13 @@ Lemma sim_skenv_monotone: forall
           (SIMSK: sim_sk ss sk_src sk_tgt)
           (LE: le ss sk_src sk_tgt ss_link)
           skenv_src skenv_tgt
-          (LESRC: SkEnv.project_spec skenv_link_src sk_src.(defs) skenv_src)
-          (LETGT: SkEnv.project_spec skenv_link_tgt sk_tgt.(defs) skenv_tgt)
+          (LESRC: SkEnv.project skenv_link_src sk_src.(defs) = skenv_src)
+          (LETGT: SkEnv.project skenv_link_tgt sk_tgt.(defs) = skenv_tgt)
         ,
           <<SIMSKENV: sim_skenv skenv_src skenv_tgt>>
 .
 Proof.
-  i.
-  inv LESRC.
-  inv LETGT.
-  inv SIMSKENV.
-  inv SIMSK. unfold match_program in *.
-  assert(DEFSEQ: sk_src.(defs) = sk_tgt.(defs)).
-  { apply Axioms.functional_extensionality. intro id.
-    hexploit (@match_program_defmap _ _ _ _ _ _ _ _ _ _ _ SIM).
-    instantiate (1:= id).
-    i.
-    inv H; ss.
-    - unfold defs.
-      admit "this is weak. add list_norept or prove my own theorem with induction.".
-    - admit "this will hold".
-  }
-  econs; eauto.
-  - eq_closure_tac.
-  - intro id.
-    destruct (Classical_Prop.classic (sk_src.(defs) id)); cycle 1.
-    + exploit SYMBDROP; eauto. i; des.
-      exploit SYMBDROP0; eauto. { rewrite <- DEFSEQ. eauto. } i; des.
-      rewrite H0. rewrite H1. ss.
-    + exploit SYMBKEEP; eauto. i; des.
-      exploit SYMBKEEP0; eauto. { rewrite <- DEFSEQ. eauto. } i; des.
-      rewrite H0. rewrite H1. ss.
-  - intro blk.
-    destruct (Genv.invert_symbol skenv_link_src blk) eqn:T0; cycle 1.
-    + rewrite DEFORPHAN; ss.
-      destruct (Genv.invert_symbol skenv_link_tgt blk) eqn:T1; cycle 1.
-      * rewrite DEFORPHAN0; ss.
-      * repeat all_once_fast ltac:(fun H => try apply Genv.invert_find_symbol in H; des).
-        rewrite <- SYMB in *.
-        repeat all_once_fast ltac:(fun H => try apply Genv.find_invert_symbol in H; des).
-        clarify.
-    + destruct (Genv.invert_symbol skenv_link_tgt blk) eqn:T1; cycle 1.
-      * repeat all_once_fast ltac:(fun H => try apply Genv.invert_find_symbol in H; des).
-        rewrite SYMB in *.
-        repeat all_once_fast ltac:(fun H => try apply Genv.find_invert_symbol in H; des).
-        clarify.
-      * repeat all_once_fast ltac:(fun H => try apply Genv.invert_find_symbol in H; des).
-        assert(i = i0).
-        { eapply Genv.genv_vars_inj; eauto. unfold Genv.find_symbol in *. rewrite SYMB. ss. }
-        clarify.
-        repeat all_once_fast ltac:(fun H => try apply Genv.find_invert_symbol in H; des).
-        destruct (classic (defs sk_src i0)).
-        { erewrite DEFKEEP; eauto. erewrite DEFKEEP0; eauto. rewrite <- DEFSEQ; ss. }
-        { erewrite DEFDROP; eauto. erewrite DEFDROP0; eauto. rewrite <- DEFSEQ; ss. }
-  - eq_closure_tac. ss. (* TODO: debug this *)
-    rewrite PUBLIC. rewrite PUBS. rewrite PUBLIC0. ss.
+  i. clarify. rr. inv SIMSK. inv SIMSKENV. ss.
 Qed.
 
 Lemma sim_skenv_func_bisim: forall
@@ -216,12 +123,12 @@ Proof.
     assert(fptr_src = fptr_tgt).
     { ss. }
     clarify. unfold Genv.find_funct, Genv.find_funct_ptr in *. des_ifs_safe.
-    erewrite <- DEFS; eauto. des_ifs. esplits; eauto.
+    esplits; eauto.
   - ii.
     assert(fptr_src = fptr_tgt).
     { ss. }
     clarify. unfold Genv.find_funct, Genv.find_funct_ptr in *. des_ifs_safe.
-    erewrite DEFS; eauto. des_ifs. esplits; eauto.
+    esplits; eauto.
 Qed.
 
 
@@ -252,11 +159,11 @@ Section REVIVE.
     clarify.
     inv SIMSKENV.
     econs; eauto.
-    ii. specialize (DEFS b). unfold SkEnv.revive. ss.
+
+    ii. ss.
     rewrite ! MapsC.PTree_filter_map_spec. rewrite ! o_bind_ignore.
-    unfold Genv.find_def in *. rewrite DEFS. des_ifs; try (by econs; eauto).
-    dup SYMB. apply find_symbol_eq_invert_symbol_eq in SYMB0. erewrite <- SYMB0.
-    destruct (Genv.invert_symbol skenv_proj_src b) eqn:T; cbn; try (by econs; eauto).
+    unfold Genv.find_def in *. des_ifs; try (by econs).
+    destruct (Genv.invert_symbol skenv_proj_tgt b) eqn:T; cbn; try (by econs; eauto).
     apply match_program_defmap with (id := i) in MATCHPROG.
     inv MATCHPROG; cbn; try (by econs; eauto).
     inv H1; ss; cycle 1.
@@ -267,3 +174,4 @@ Section REVIVE.
   Qed.
 
 End REVIVE.
+
